examples/algorithms/GenericStability.fst
@@ -33,89 +33,78 @@ let rec filter_eq_contains #a k xs key =
   | hd::tl ->
     filter_eq_contains k tl key
 
-val filter_eq_append: #a:eqtype -> (x:int) -> (l1: list a) -> (l2: list a) -> k:(a -> Tot int) ->
-  Lemma(ensures((filter_eq x l1 k)@(filter_eq x l2 k) = filter_eq x (l1@l2) k))
-let rec filter_eq_append #a x l1 l2 k =
+val filter_eq_append: #a:eqtype -> (l1: list a) -> (l2: list a) -> k:(a -> Tot int) ->
+  Lemma(ensures(forall x. (filter_eq x l1 k)@(filter_eq x l2 k) = filter_eq x (l1@l2) k))
+let rec filter_eq_append #a l1 l2 k =
   match l1 with
   | [] -> ()
   | hd::tl ->
-    filter_eq_append x tl l2 k
+    filter_eq_append tl l2 k
 
-val filter_eq_not_contains: #a:eqtype -> (x:int) -> (l: list a) -> k:(a -> Tot int) ->
-  Lemma(ensures (filter_eq x l k) = [] <==> ~(exists e. (mem e l /\ k e = x)))
-let rec filter_eq_not_contains #a x l k =
+val filter_eq_not_contains: #a:eqtype -> (l: list a) -> k:(a -> Tot int) ->
+  Lemma(ensures (forall x. (filter_eq x l k) = [] <==> ~(exists e. (mem e l /\ k e = x))))
+let rec filter_eq_not_contains #a l k =
   match l with
   | [] -> ()
   | hd::tl ->
-    filter_eq_not_contains x tl k;
-    mem_existsb (fun y -> k y = x) l
-
-val is_stable: #a:eqtype -> int -> list a -> list a -> (a -> Tot int) -> Tot bool
-let is_stable #a x l1 l2 k = (filter_eq x l1 k = filter_eq x l2 k)
-
-type stable (#a:eqtype) (l1:list a) (l2:list a) = forall x k. is_stable x l1 l2 k
+    filter_eq_not_contains tl k
 
 val filter_eq_single: #a:eqtype ->
-  (x:int) ->
   (l: list a{is_Cons l /\ length l = 1}) ->
   k:(a -> Tot int) ->
-  Lemma(ensures((k (hd l) = x ) ==> filter_eq x l k = [hd l]))
-let filter_eq_single #a x l k = ()
+  Lemma(ensures(forall x. (k (hd l) = x ) ==> filter_eq x l k = [hd l]))
+let filter_eq_single #a l k = ()
 
-val filter_eq_sorted_lt:  #a:eqtype -> x: int -> l:list a{is_Cons l} -> k:(a -> Tot int) ->
-  Lemma(requires (sorted l k /\ x < k (hd l)))
-  (ensures(filter_eq x l k = []))
-let filter_eq_sorted_lt #a x l k =
-  sorted_lt x l k;
-  filter_eq_not_contains x l k
-
+val filter_eq_sorted_lt:  #a:eqtype -> l:list a{is_Cons l} -> k:(a -> Tot int) ->
+  Lemma(requires (sorted l k))
+  (ensures(forall x. (x < k (hd l)) ==> (filter_eq x l k = [])))
+let filter_eq_sorted_lt #a l k =
+  sorted_lt l k;
+  filter_eq_not_contains l k
 
 val filter_eq_first: #a:eqtype ->
-  (x:int) ->
   (l1: list a{is_Cons l1}) ->
   (l2: list a{is_Cons l2}) ->
   k:(a -> Tot int) ->
-  Lemma(requires (sorted l1 k) /\ (k (hd l2) = x ) /\  (k (hd l1) > k (hd l2)))
-  (ensures (k (hd l2) = x ) ==> filter_eq x (l1@l2) k = ((filter_eq x ((hd l2)::l1) k )@(filter_eq x (tl l2) k)))
-let filter_eq_first #a x l1 l2 k =
-  filter_eq_append x l1 l2 k;
-  filter_eq_sorted_lt x l1 k
+  Lemma(requires (sorted l1 k) /\  (k (hd l1) > k (hd l2)))
+  (ensures (forall x. (k (hd l2) = x ) ==>
+    filter_eq x (l1@l2) k = ((filter_eq x ((hd l2)::l1) k )@(filter_eq x (tl l2) k))))
+let filter_eq_first #a l1 l2 k =
+  filter_eq_append l1 l2 k;
+  filter_eq_sorted_lt l1 k
+
+type stable (#a:eqtype) (l1:list a) (l2:list a) (k:(a -> Tot int)) = forall x. (filter_eq x l1 k = filter_eq x l2 k)
 
 val stable_lift: #a:eqtype ->
-  (x:int) ->
   (l1: list a{is_Cons l1}) ->
   (l2: list a{is_Cons l2}) ->
   k:(a -> Tot int) ->
   Lemma(requires (sorted l1 k) /\ (k (hd l1) > k (hd l2)))
-  (ensures (is_stable x (l1@l2) (((hd l2)::l1)@(tl l2)) k))
-let stable_lift #a x l1 l2 k =
-  filter_eq_append x l1 l2 k;
-  append_assoc (filter_eq x l1 k) (filter_eq x [hd l2] k) (filter_eq x (tl l2) k);
-  if (k (hd l2) = x) then(
-    filter_eq_append x ((hd l2)::l1) (tl l2) k;
-    filter_eq_first x l1 l2 k)
-  else filter_eq_append x ((hd l2)::l1) (tl l2) k
+  (ensures (stable (l1@l2) (((hd l2)::l1)@(tl l2)) k))
+let stable_lift #a l1 l2 k =
+  filter_eq_append l1 l2 k;
+  filter_eq_append ((hd l2)::l1) (tl l2) k;
+  filter_eq_first l1 l2 k;
+  filter_eq_append ((hd l2)::l1) (tl l2) k
 
 val stable_append_l: #a:eqtype ->
-  (x:int) ->
   (l: list a) ->
   (r: list a) ->
   (r': list a) ->
   k:(a -> Tot int) ->
-  Lemma(ensures(is_stable x r r' k ==> is_stable x (l@r) (l@r') k))
-let rec stable_append_l #a x l r r' k =
+  Lemma(ensures(stable r r' k ==> stable (l@r) (l@r') k))
+let rec stable_append_l #a l r r' k =
   match l with
   | [] -> ()
-  | hd::tl -> stable_append_l x tl r r' k
+  | hd::tl -> stable_append_l tl r r' k
 
 val stable_append_r: #a:eqtype ->
-  (x:int) ->
   (l: list a) ->
   (l': list a) ->
   (r: list a) ->
   k:(a -> Tot int) ->
-  Lemma(requires(is_stable x l l' k))
-  (ensures(is_stable x (l@r) (l'@r) k))
-let rec stable_append_r #a x l l' r k =
-  filter_eq_append x l r k;
-  filter_eq_append x l' r k
+  Lemma(requires(stable l l' k))
+  (ensures(stable (l@r) (l'@r) k))
+let rec stable_append_r #a l l' r k =
+  filter_eq_append l r k;
+  filter_eq_append l' r k
