examples/algorithms/MergeSort2.fst
@@ -12,7 +12,6 @@ open GenericSort
 open GenericStability
 (**
   The key function k will appear frequently here.
-  As will x, a value that some list is filtered for.
 **)
 
 (** First define the merge function without any properties.**)
@@ -66,26 +65,26 @@ val merge'_nil_r: #a:eqtype -> (r: list a) -> k:(a -> Tot int) ->
 let merge'_nil_r #a r k = ()
 
 (** filtering (l appended to r) wrt x is equivelant to merging l and r, then filtering wrt x **)
-val merge'_filter_eq_inv: #a:eqtype -> (x:int) -> (l: list a{is_Cons l}) -> (r: list a{is_Cons r}) -> k:(a -> Tot int) ->
+val merge'_filter_eq_inv: #a:eqtype -> (l: list a{is_Cons l}) -> (r: list a{is_Cons r}) -> k:(a -> Tot int) ->
   Lemma(requires (sorted l k /\ sorted r k))
-    (ensures ((is_Cons l /\ is_Cons r)/\(filter_eq x (l@r) k = filter_eq x (merge' l r k) k)))
-let rec merge'_filter_eq_inv #a x l r k =
+    (ensures (forall x. ((is_Cons l /\ is_Cons r)/\ (filter_eq x (l@r) k = filter_eq x (merge' l r k) k))))
+let rec merge'_filter_eq_inv #a l r k =
   if k (hd r) < k (hd l) then
-    (stable_lift x l r k;
+    (stable_lift l r k;
     merge'_hd l r k;
     if (tl r) = [] then merge'_l_nil l k
-    else (merge'_filter_eq_inv x l (tl r) k;
-      filter_eq_append x [hd r] (merge' l (tl r) k) k))
+    else (merge'_filter_eq_inv l (tl r) k;
+      filter_eq_append [hd r] (merge' l (tl r) k) k))
   else (merge'_hd l r k;
     if (tl l) = [] then (merge'_nil_r r k)
-    else (merge'_filter_eq_inv x (tl l) r k;
-      filter_eq_append x [hd l] (merge' (tl l) r k) k))
+    else (merge'_filter_eq_inv (tl l) r k;
+      filter_eq_append [hd l] (merge' (tl l) r k) k))
 
 (** merge is stable **)
-val merge'_stable: #a:eqtype -> x:int -> (l: list a{is_Cons l}) -> (r: list a{is_Cons r}) -> k:(a -> Tot int) ->
+val merge'_stable: #a:eqtype -> (l: list a{is_Cons l}) -> (r: list a{is_Cons r}) -> k:(a -> Tot int) ->
   Lemma(requires (sorted l k /\ sorted r k))
-  (ensures is_stable x (l@r) (merge' l r k) k)
-let merge'_stable #a x l r k = merge'_filter_eq_inv x l r k
+  (ensures stable (l@r) (merge' l r k) k)
+let merge'_stable #a l r k = merge'_filter_eq_inv l r k
 
 (** Define mergesort, and show that it returns a sorted list **)
 val mergesort': #a:eqtype -> l:list a -> k:(a -> Tot int) -> Tot (l':list a{sorted l' k})
@@ -97,16 +96,16 @@ let rec mergesort' #a l k =
     merge' (merge' [a] [b] k) (mergesort' tl k) k
 
 (** Mergesort is stable **)
-val mergesort'_stable': #a:eqtype -> x:int -> l:list a -> k:(a -> Tot int) ->
-  Lemma(ensures (is_stable x (mergesort' l k) l k))
-let rec mergesort'_stable' #a x l k =
+val mergesort'_stable': #a:eqtype -> l:list a -> k:(a -> Tot int) ->
+  Lemma(ensures (stable (mergesort' l k) l k))
+let rec mergesort'_stable' #a l k =
   match l with
   | [] | [_] -> ()
   | a::b::tl ->
-    if tl = [] then merge'_stable x [a] [b] k
+    if tl = [] then merge'_stable [a] [b] k
     else
-      merge'_stable x (merge' [a] [b] k) (mergesort' tl k) k;
-      mergesort'_stable' x tl k
+      merge'_stable (merge' [a] [b] k) (mergesort' tl k) k;
+      mergesort'_stable' tl k
 
 (** Mergesort returns a permutation of l**)
 val mergesort'_permutation: #a:eqtype -> l:list a -> k:(a -> Tot int) ->
@@ -121,14 +120,10 @@ let rec mergesort'_permutation #a l k =
       merge'_permutation (merge' [a] [b] k) (mergesort' tl k) k;
       mergesort'_permutation tl k
 
-(*
-  Ideally, I'd like to type mergesort as stable rather than use is_stable.
-*)
-
 (** Finally, we define mergesort and prove it's properties**)
-val mergesort: #a:eqtype -> x:int -> l:list a -> k:(a -> Tot int) ->
-  Tot (l':list a{sorted l' k /\ permutation l l' /\ (is_stable x l' l k)})
-let mergesort #a x l k =
+val mergesort: #a:eqtype -> l:list a -> k:(a -> Tot int) ->
+  Tot (l':list a{sorted l' k /\ permutation l l' /\ (stable l' l k)})
+let mergesort #a l k =
   mergesort'_permutation l k;
-  mergesort'_stable' x l k;
+  mergesort'_stable' l k;
   mergesort' l k
